timing/examples/FreeRTOS/list/uxListRemove.v
@@ -1,0 +1,131 @@
+Require Import RTOSDemo_NoAsserts_Clz.
+Require Import riscvTiming.
+Import RISCVNotations.
+Require Import timing_auto.
+
+Variable ML : N.
+Variable ML_pos : 1 <= ML.
+
+Definition time_mem : N :=
+    5 + (ML - 2).
+Definition time_branch : N :=
+    5 + (ML - 1).
+
+Module uxListRemoveTime <: TimingModule.
+    Definition time_of_addr (s : store) (a : addr) : N :=
+        match neorv32_cycles_upper_bound ML s (RTOSDemo_NoAsserts_Clz a) with
+        | Some x => x | _ => 999 end.
+
+    Definition entry_addr : N := 0x80002440.
+
+    Definition exits (t:trace) : bool :=
+    match t with (Addr a,_)::_ => match a with
+    | 0x80002470 => true
+    | _ => false
+  end | _ => false end.
+End uxListRemoveTime.
+
+Module uxListRemoveAuto := TimingAutomation uxListRemoveTime.
+Import uxListRemoveTime uxListRemoveAuto.
+
+Definition time_of_uxListRemove (t : trace) (base_mem : addr -> N) (a0 : N) :=
+    cycle_count_of_trace t = 6 * time_mem +
+        (if base_mem Ⓓ[4 + base_mem Ⓓ[16 + a0]] =? a0 then 3 + time_mem else time_branch) + 
+        3 * time_mem + 2 + time_branch.
+
+(* https://github.com/FreeRTOS/FreeRTOS-Kernel/blob/main/include/list.h#L143 *)
+Definition xItemValue (mem : addr -> N) (list_item_addr : addr) : N :=
+    mem Ⓓ[list_item_addr].
+Definition pxNext (mem : addr -> N) (list_item_addr : addr) : addr :=
+    mem Ⓓ[4 + list_item_addr].
+Definition pxPrevious (mem : addr -> N) (list_item_addr : addr) : addr :=
+    mem Ⓓ[8 + list_item_addr].
+Definition pxContainer (mem : addr -> N) (list_item_addr : addr) : addr :=
+    mem Ⓓ[16 + list_item_addr].
+
+Definition pxIndex (mem : addr -> N) (list_addr : addr) : N :=
+    mem Ⓓ[4 + list_addr].
+
+Definition noverlaps (mem : addr -> N) (a0 : N) :=
+    let regions := map (fun x => (4, x)) 
+        [4 + a0; 8 + a0; 16 + a0;
+         4 + (pxPrevious mem a0); 8 + (pxNext mem a0);
+         4 + (pxContainer mem a0)] in
+    create_noverlaps regions regions.
+
+Definition uxListRemove_timing_invs (base_mem : addr -> N) (a0 : N)
+    (t:trace) : option Prop :=
+match t with (Addr a, s) :: t' => match a with
+| 0x80002440 => Some (s R_A0 = Ⓓa0 /\ s V_MEM32 = Ⓜbase_mem /\
+                        noverlaps base_mem a0 /\
+                        cycle_count_of_trace t' = 0)
+| 0x80002460 => Some (exists mem, s V_MEM32 = Ⓜmem /\
+                        noverlaps mem a0 /\
+                        cycle_count_of_trace t' = 6 * time_mem +
+                            (if base_mem Ⓓ[4 + base_mem Ⓓ[16 + a0]] =? a0 then 3 + time_mem else time_branch))
+| 0x80002470 => Some (exists mem, s V_MEM32 = Ⓜmem /\ 
+                        time_of_uxListRemove t base_mem a0)
+| _ => None end | _ => None end.
+
+Definition lifted_uxListRemove : program :=
+    lift_riscv RTOSDemo_NoAsserts_Clz.
+
+(* We use simpl in a few convenient places: make sure it doesn't go haywire *)
+Arguments N.add _ _ : simpl nomatch.
+Arguments N.mul _ _ : simpl nomatch.
+
+Theorem uxListRemove_timing:
+  forall s t s' x' base_mem a0
+         (ENTRY: startof t (x',s') = (Addr entry_addr, s))
+         (MDL: models rvtypctx s)
+         (NVL : noverlaps base_mem a0)
+         (MEM: s V_MEM32 = Ⓜbase_mem)
+         (A0: s R_A0 = Ⓓa0),
+  satisfies_all 
+    lifted_uxListRemove
+    (uxListRemove_timing_invs base_mem a0)
+    exits
+  ((x',s')::t).
+Proof using.
+    intros.
+    apply prove_invs.
+    Local Ltac step := time rv_step.
+    Local Ltac unfold_noverlap :=
+        unfold pxNext, pxPrevious, pxContainer, pxIndex, noverlaps in *.
+    Local Ltac preserve_noverlaps := 
+        noverlaps_preserved unfold_noverlap.
+
+    simpl. rewrite ENTRY. unfold entry_addr. step.
+    auto.
+
+    intros.
+    eapply startof_prefix in ENTRY; try eassumption.
+    eapply preservation_exec_prog in MDL; 
+        try eassumption; [idtac|apply lift_riscv_welltyped].
+    clear - ENTRY PRE MDL. rename t1 into t. rename s1 into s'.
+
+    destruct_inv 32 PRE.
+
+    destruct PRE as (cycles & A0 & NVL & MEM).
+    repeat step. {
+        eexists. split. reflexivity. split.
+            preserve_noverlaps.
+        hammer. find_rewrites. unfold_create_noverlaps unfold_noverlap.
+        rewrite getmem_noverlap, getmem_noverlap in BC by auto.
+        apply Bool.negb_true_iff in BC. rewrite BC. unfold time_mem, time_branch.
+        psimpl. lia.
+    } {
+        eexists. split. reflexivity. split.
+            preserve_noverlaps.
+        hammer. find_rewrites. unfold_create_noverlaps unfold_noverlap.
+        rewrite getmem_noverlap, getmem_noverlap in BC by auto.
+        apply Bool.negb_false_iff in BC. rewrite BC. unfold time_mem, time_branch.
+        psimpl. lia.
+    }
+
+    destruct PRE as (mem & MEM & NVL & Cycles).
+    repeat step. eexists. split. reflexivity.
+    unfold time_of_uxListRemove. hammer. find_rewrites. psimpl.
+    unfold time_mem, time_branch. psimpl. destruct N.eqb; psimpl; lia.
+Qed.
+
