timing/timing_auto.v
@@ -1,0 +1,75 @@
+Require Import riscvTiming.
+Require Export List.
+Export ListNotations.
+
+Module Type TimingModule.
+    Parameter time_of_addr : store -> addr -> N.
+    Parameter entry_addr : N.
+    Parameter exits : trace -> bool.
+End TimingModule.
+
+Module TimingAutomation (tm : TimingModule).
+
+Export Lia.
+
+Definition cycle_count_of_trace := cycle_count_of_trace tm.time_of_addr.
+
+Ltac unfold_decompose :=
+    cbv [decompose_Btype decompose_Itype decompose_Jtype decompose_Rtype 
+        decompose_Stype decompose_Utype mask_bit_section]; cbn [N.land].
+Tactic Notation "unfold_decompose" "in" hyp(H) :=
+    cbv [decompose_Btype decompose_Itype decompose_Jtype decompose_Rtype 
+        decompose_Stype decompose_Utype mask_bit_section] in H; cbn [N.land] in H.
+Ltac unfold_time_of_addr :=
+    cbv [tm.time_of_addr neorv32_cycles_upper_bound]; cbn - [setmem getmem].
+Tactic Notation "unfold_time_of_addr" "in" hyp(H) :=
+    cbv [tm.time_of_addr neorv32_cycles_upper_bound] in H; cbn - [setmem getmem].
+Ltac unfold_cycle_count_list :=
+    unfold cycle_count_of_trace; repeat rewrite cycle_count_of_trace_cons, cycle_count_of_trace_single; fold cycle_count_of_trace.
+Ltac hammer :=
+    unfold_cycle_count_list; unfold_time_of_addr; unfold_decompose; psimpl; try lia.
+
+Ltac find_rewrites :=
+    repeat (match goal with
+    | [H: ?x = _ |- context[match ?x with _ => _ end]] =>
+        rewrite H
+    | [H: ?x = _ |- context[if ?x then _ else _]] =>
+        rewrite H
+    | [H: cycle_count_of_trace ?t = _ |- context[cycle_count_of_trace ?t]] =>
+        rewrite H
+    end).
+
+Ltac handle_ex := 
+    repeat (match goal with
+    | [|- exists _, _] => eexists
+    end); repeat split; try eassumption.
+
+End TimingAutomation.
+
+(* Memory layout *)
+Fixpoint create_noverlaps (l l' : list (N * addr)) : Prop :=
+    match l' with
+    | [] => True
+    | (size, addr) :: t => (fold_left 
+        (fun P item => 
+            match item with (size', addr') =>
+            P /\ ~ overlap 32 addr size addr' size'
+            end) l True) /\ create_noverlaps l t
+    end.
+
+Ltac unfold_create_noverlaps unfolds :=
+    unfolds;
+    match goal with
+    | [H: create_noverlaps _ _ |- _] =>
+        unfold create_noverlaps in H; cbn [map fold_left] in H;
+        repeat (match goal with [H: _ /\ _ |- _] => destruct H end)
+    | [H: let _ := _ in create_noverlaps _ _ |- _] =>
+        unfold create_noverlaps in H; cbn [map fold_left] in H;
+        repeat (match goal with [H: _ /\ _ |- _] => destruct H end)
+    end;
+    repeat match goal with [H: True |- _] => clear H end.
+
+Ltac noverlaps_preserved unfolds :=
+    solve [unfold_create_noverlaps unfolds; unfolds;
+           repeat split;
+           repeat rewrite getmem_noverlap; auto].
